SSA/Experimental/IntrinsicAsymptotics/Lets.lean
@@ -1,0 +1,78 @@
+import SSA.Experimental.IntrinsicAsymptotics.Context
+
+def Ctxt.IsVarOfType (Γ : Ctxt) (n : Nat) (t: Ty) : Prop :=
+  Γ.out.get? n = some t
+
+/-- A very simple expression, without type information. -/
+inductive ExprRaw : Type
+  | add : Nat → Nat → ExprRaw
+  /-- Nat literals. -/
+  | nat : Nat → ExprRaw
+
+/-- A recursive expression, without type information. -/
+inductive ExprRecRaw : Type
+  | add : ExprRecRaw → ExprRecRaw → ExprRecRaw
+  /-- Nat literals -/
+  | nat : Nat → ExprRecRaw
+  /-- Free/meta variables -/
+  | var : Nat → ExprRecRaw
+
+
+inductive ExprRaw.IsWellTyped (Γ : Ctxt) : Ty → ExprRaw → Prop
+  | add {v w : Nat} : Γ.IsVarOfType v .nat → Γ.IsVarOfType w .nat → IsWellTyped Γ .nat (.add v w)
+  | nat {n : Nat} : IsWellTyped Γ .nat (.nat n)
+
+inductive ExprRecRaw.IsWellTyped (Γ : Ctxt) : Ty → ExprRecRaw → Prop
+  | add {e₁ e₂ : ExprRecRaw} : IsWellTyped Γ .nat e₁ → IsWellTyped Γ .nat e₂ → IsWellTyped Γ .nat (.add e₁ e₂)
+  | nat {n : Nat} : IsWellTyped Γ .nat (.nat n)
+
+inductive Lets.IsWellTyped : Ctxt → Ctxt → List ExprRaw → Prop
+  | nil   : IsWellTyped Γ Γ []
+  | lete  : IsWellTyped Γin Γout lets → ExprRaw.IsWellTyped Γout t e 
+            → IsWellTyped Γin (Γout.snoc t) (e :: lets)
+
+
+
+
+structure IExpr (Γ : Ctxt) (t : Ty) where
+  raw : ExprRaw
+  wt : raw.IsWellTyped Γ t
+
+structure IExprRec (Γ : Ctxt) (t : Ty) where
+  raw : ExprRecRaw
+  wt : raw.IsWellTyped Γ t
+
+
+structure Lets (Γ_in Γ_out : Ctxt) where
+  raw : Array ExprRaw
+  wt : Lets.IsWellTyped Γ_in Γ_out raw.1.reverse
+
+
+def Lets.snocLet (lets : Lets Γi Γo) (e : IExpr Γo t) : Lets Γi (Γo.snoc t) where 
+  raw := lets.raw.push e.raw
+  wt  := by
+    simp only [Array.push, Array.data, List.concat_eq_append, List.reverse_append, 
+                List.reverse_cons, List.reverse_nil, List.nil_append, List.singleton_append]
+    exact IsWellTyped.lete lets.wt e.wt
+
+def Lets.size : Lets Γi Γo → Nat :=
+  Array.size ∘ Lets.raw  
+
+def Lets.IsWellTyped.wtTail : IsWellTyped Γ 
+
+def Lets.outContext (lets : Lets Γi Γo) : { Δ : Ctxt // Γo = Γi ++ Δ} :=
+  go _ lets.raw.1.reverse lets.wt
+where
+  go (Γo' : Ctxt) : (lets : List ExprRaw) → IsWellTyped Γi Γo' lets → { Δ : Ctxt // Γo' = Γi ++ Δ}
+    | [], wt => ⟨∅, by cases wt; simp⟩
+    | e::lets, wt => 
+        let Γo' : Ctxt := by 
+          cases Γo'
+          next => exfalso; cases wt
+        let r := go Γo' lets (by cases wt; next wt => exact wt)
+        _
+
+def Lets.get (lets : Lets Γi Γo) (v : Γo.Var t) : 
+    Option ((Γo' : Ctxt) × (Γo'.hom Γo) × IExpr Γo' t) :=
+    
+  
